theories/lang/int_type.v
@@ -62,7 +62,8 @@ Definition uintptr_t := IntType bytes_per_addr_log false.
 Definition size_t  := uintptr_t.
 Definition ssize_t := intptr_t.
 Definition ptrdiff_t := intptr_t.
-Definition bool_it := u8.
+
+Definition bool_layout : layout := {| ly_size := 1; ly_align_log := 0 |}.
 
 (*** Lemmas about [int_type] *)
 
